compiler/proofs/patLangProofScript.sml
@@ -141,36 +141,6 @@ val map_count_store_genv_def = Define`
   map_count_store_genv f (csg:'a count_store_genv) =
     ((FST(FST csg), MAP f (SND(FST csg))), MAP (OPTION_MAP f) (SND csg))`
 
-val csg_rel_def = Define`
-  csg_rel R ((c1,s1),g1) (((c2,s2),g2):'a count_store_genv) ⇔
-    c1 = c2 ∧ LIST_REL R s1 s2 ∧ LIST_REL (OPTION_REL R) g1 g2`
-
-val csg_rel_refl = store_thm("csg_rel_refl",
-  ``∀V x. (∀x. V x x) ⇒ csg_rel V x x``,
-  rpt gen_tac >> PairCases_on`x` >> simp[csg_rel_def] >>
-  rw[] >> match_mp_tac EVERY2_refl >>
-  rw[optionTheory.OPTREL_def] >>
-  Cases_on`x` >> rw[])
-val _ = export_rewrites["csg_rel_refl"]
-
-val csg_rel_trans = store_thm("csg_rel_trans",
-  ``∀V. (∀x y z. V x y ∧ V y z ⇒ V x z) ⇒ ∀x y z. csg_rel V x y ∧ csg_rel V y z ⇒ csg_rel V x z``,
-  rw[] >> map_every PairCases_on [`x`,`y`,`z`] >>
-  fs[csg_rel_def] >>
-  conj_tac >>
-  match_mp_tac (MP_CANON EVERY2_trans)
-  >- metis_tac[] >>
-  simp[optionTheory.OPTREL_def] >>
-  qexists_tac`y2` >> simp[] >>
-  Cases >> Cases >> Cases >> simp[] >>
-  metis_tac[])
-
-val csg_rel_count = store_thm("csg_rel_count",
-  ``csg_rel R csg1 csg2 ⇒ FST(FST csg2) = FST(FST csg1)``,
-  PairCases_on`csg1` >>
-  PairCases_on`csg2` >>
-  simp[csg_rel_def])
-
 (* --- *)
 
 (* TODO: move *)
