compiler/proofs/printingScript.sml
@@ -1,0 +1,694 @@
+open HolKernel boolLib boolSimps bossLib lcsymtacs listTheory stringTheory relationTheory rich_listTheory pairTheory arithmeticTheory finite_mapTheory
+open miscLib miscTheory bytecodeTheory bytecodeExtraTheory bytecodeEvalTheory bytecodeLabelsTheory bytecodeTerminationTheory
+open intLangTheory intLangExtraTheory toBytecodeTheory compilerTheory compilerTerminationTheory
+open modLangProofTheory conLangProofTheory exhLangProofTheory patLangProofTheory intLangProofTheory bytecodeProofTheory free_varsTheory 
+open replTheory terminationTheory
+
+val _ = new_theory"printing"
+
+(* TODO: move? *)
+
+val FOLDL_emit_thm = store_thm("FOLDL_emit_thm",
+  ``∀ls s. FOLDL (λs i. s with out := i::s.out) s ls = s with out := REVERSE ls ++ s.out``,
+  Induct >> simp[compiler_result_component_equality])
+
+(* value refinement *)
+
+val exh_Cv_def = Define`
+  exh_Cv v Cv ⇔
+    ∃vp. v_pat (v_to_pat v) vp ∧ closed_pat vp ∧ syneq (v_to_Cv vp) Cv`
+
+val v_bv_def = Define`
+  v_bv (genv,gtagenv,exh,pp) v bv ⇔
+    ∃v1 v2 vh Cv.
+    v_to_i1 genv v v1 ∧
+    v_to_i2 gtagenv v1 v2 ∧
+    v_to_exh exh v2 vh ∧
+    exh_Cv vh Cv ∧
+    Cv_bv pp Cv bv`
+
+val exh_Cv_syneq_trans = store_thm("exh_Cv_syneq_trans",
+  ``∀v Cv Cv2. exh_Cv v Cv ∧ syneq Cv Cv2 ⇒ exh_Cv v Cv2``,
+  rw[exh_Cv_def] >> metis_tac[syneq_trans])
+
+val LIST_REL_exh_Cv_syneq_trans = store_thm("LIST_REL_exh_Cv_syneq_trans",
+  ``∀vs Cvs Cvs2.
+    LIST_REL syneq Cvs Cvs2
+    ∧
+    LIST_REL (exh_Cv) vs Cvs
+    ⇒
+    LIST_REL (exh_Cv) vs Cvs2``,
+  rw[EVERY2_EVERY,EVERY_MEM] >> rfs[MEM_ZIP,PULL_EXISTS] >>
+  metis_tac[exh_Cv_syneq_trans])
+
+val LIST_REL_OPTREL_exh_Cv_syneq_trans = store_thm("LIST_REL_OPTREL_exh_Cv_syneq_trans",
+  ``∀vs Cvs Cvs2.
+    LIST_REL (OPTREL syneq) Cvs Cvs2
+    ∧
+    LIST_REL (OPTREL (exh_Cv)) vs Cvs
+    ⇒
+    LIST_REL (OPTREL (exh_Cv)) vs Cvs2``,
+  rw[EVERY2_EVERY,EVERY_MEM] >> rfs[MEM_ZIP,PULL_EXISTS] >>
+  fs[optionTheory.OPTREL_def] >>
+  metis_tac[exh_Cv_syneq_trans,optionTheory.SOME_11,optionTheory.NOT_SOME_NONE])
+
+(* printing *)
+
+val _ = Parse.overload_on("print_bv",``λx. ov_to_string (bv_to_ov x)``)
+val print_bv_str_def = Define`print_bv_str t v w = "val "++v++":"++(tystr t v)++" = "++(print_bv w)++"\n"`
+
+val append_cons_lemma = prove(``ls ++ [x] ++ a::b = ls ++ x::a::b``,lrw[])
+
+val MAP_PrintC_thm = store_thm("MAP_PrintC_thm",
+  ``∀ls bs bc0 bc1 bs'.
+    bs.code = bc0 ++ (MAP PrintC ls) ++ bc1 ∧
+    bs.pc = next_addr bs.inst_length bc0 ∧
+    bs' = bs with <| output := bs.output ++ ls; pc := next_addr bs.inst_length (bc0 ++ (MAP PrintC ls))|>
+    ⇒
+    bc_next^* bs bs'``,
+  Induct >- (
+    simp[] >> rw[] >>
+    simp[Once RTC_CASES1] >> disj1_tac >>
+    simp[bc_state_component_equality] ) >>
+  simp[] >> rw[] >>
+  simp[Once RTC_CASES1] >> disj2_tac >>
+  `bc_fetch bs = SOME (PrintC h)` by (
+    match_mp_tac bc_fetch_next_addr >>
+    qexists_tac`bc0` >>
+    simp[] ) >>
+  simp[bc_eval1_thm,bc_eval1_def,bump_pc_def] >>
+  first_x_assum match_mp_tac >>
+  simp[bc_state_component_equality,IMPLODE_EXPLODE_I] >>
+  qexists_tac`bc0 ++ [PrintC h]` >>
+  simp[FILTER_APPEND,SUM_APPEND])
+
+val _ = Parse.overload_on("print_bv_list",``λt vs ws. FLAT (MAP (UNCURRY (print_bv_str t)) (ZIP (vs,ws)))``)
+
+val print_envE_cons = store_thm("print_envE_cons",
+  ``print_envE types (x::xs) = print_envE types [x]++print_envE types xs``,
+  rw[print_envE_def]);
+
+val print_v_ov = prove(
+  ``(∀genv v v1. v_to_i1 genv v v1 ⇒
+      ∀gtagenv v2 exh vh Cv.
+        v_to_i2 gtagenv v1 v2 ∧
+          v_to_exh exh v2 vh ∧ exh_Cv vh Cv ⇒
+            ov_to_string (Cv_to_ov Cv) = print_v v) ∧
+    (∀genv vs vs1. vs_to_i1 genv vs vs1 ⇒ T) ∧
+    (∀genv env env1. env_to_i1 genv env env1 ⇒ T) ∧
+    (∀genv map sh env. global_env_inv_flat genv map sh env ⇒ T) ∧
+    (∀genv mods tops menv sh env. global_env_inv genv mods tops menv sh env ⇒ T)``,
+  ho_match_mp_tac v_to_i1_ind >> simp[] >> rpt conj_tac >>
+  TRY (
+    simp[Once v_to_i2_cases,exh_Cv_def] >> rw[] >>
+    simp[printerTheory.ov_to_string_def,print_v_def] >>
+    Cases_on`lit`>>simp[printerTheory.ov_to_string_def,print_v_def,print_lit_def] >>
+    Cases_on`b`>>simp[printerTheory.ov_to_string_def,print_v_def,print_lit_def] ) >>
+  simp[Once v_to_i2_cases] >>
+  rw[] >> fs[exh_Cv_def] >>
+  rator_x_assum`v_to_exh`mp_tac >>
+  rw[Once v_to_exh_cases,PULL_EXISTS] >>
+  rator_x_assum`v_pat`mp_tac >>
+  rw[Once v_pat_cases,PULL_EXISTS] >>
+  rator_x_assum`syneq`mp_tac >>
+  rw[Once syneq_cases,PULL_EXISTS,LET_THM] >>
+  simp[print_v_def,printerTheory.ov_to_string_def])
+val print_v_ov = save_thm("print_v_ov",CONJUNCT1 print_v_ov)
+
+val print_bv_list_print_envE = store_thm("print_bv_list_print_envE",
+  ``∀bvs types vars env data.
+    vars = MAP FST env ∧
+    LIST_REL (v_bv data) (MAP SND env) bvs ∧
+    set vars ⊆ FDOM types
+    ⇒
+    print_bv_list types vars bvs = print_envE types env``,
+  Induct_on`env` >- ( simp[print_envE_def] ) >>
+  qx_gen_tac`x`>>PairCases_on`x` >> simp[PULL_EXISTS] >>
+  rpt gen_tac >> strip_tac >> fs[] >>
+  fs[GSYM AND_IMP_INTRO] >>
+  first_x_assum(fn th => first_x_assum(strip_assume_tac o MATCH_MP th)) >>
+  first_x_assum(fn th => first_x_assum(strip_assume_tac o MATCH_MP th)) >>
+  simp[print_envE_def,print_bv_str_def] >> simp[tystr_def,FLOOKUP_DEF] >>
+  PairCases_on`data` >> fs[v_bv_def] >>
+  first_x_assum(mp_tac o MATCH_MP print_v_ov) >>
+  simp[GSYM AND_IMP_INTRO] >>
+  disch_then(fn th => first_x_assum (mp_tac o MATCH_MP th)) >>
+  disch_then(fn th => first_x_assum (mp_tac o MATCH_MP th)) >>
+  metis_tac[Cv_bv_ov])
+
+val code_labels_ok_MAP_PrintC = store_thm("code_labels_ok_MAP_PrintC",
+  ``∀ls. code_labels_ok (MAP PrintC ls)``,
+  Induct>>simp[]>>rw[]>>match_mp_tac code_labels_ok_cons>>simp[])
+val _ = export_rewrites["code_labels_ok_MAP_PrintC"]
+
+val can_Print_list_EVERY = store_thm("can_Print_list_EVERY",
+  ``∀ls. can_Print_list ls = EVERY can_Print ls``,
+  Induct >> simp[])
+val _ = export_rewrites["can_Print_list_EVERY"]
+
+val compile_print_vals_thm = store_thm("compile_print_vals_thm",
+  ``∀vs types map cs. let cs' = compile_print_vals types map vs cs in
+    ∃code. cs'.out = REVERSE code ++ cs.out
+         ∧ cs'.next_label = cs.next_label
+         ∧ EVERY ($~ o is_Label) code ∧
+         code_labels_ok code ∧
+    ∀bs bc0 bvs.
+    bs.code = bc0 ++ code
+    ∧ bs.pc = next_addr bs.inst_length bc0
+    ∧ LIST_REL (λv bv. ∃n. FLOOKUP map v = SOME n ∧ el_check n bs.globals = SOME (SOME bv) ∧ can_Print bv) vs bvs
+    ⇒
+    let bs' = bs with <|pc := next_addr bs.inst_length (bc0++code)
+                       ;output := bs.output ++ print_bv_list types vs bvs|> in
+    bc_next^* bs bs'``,
+  Induct >> simp[compile_print_vals_def] >- (
+    simp[Once SWAP_REVERSE] >> rw[] >>
+    simp[Once RTC_CASES1] >>
+    simp[bc_state_component_equality] )>>
+  simp[FOLDL_emit_thm] >>
+  qx_gen_tac`v` >>
+  rpt strip_tac >>
+  Q.PAT_ABBREV_TAC`cs1 = compiler_result_out_fupd X Y` >>
+  first_x_assum(qspecl_then[`types`,`map`,`cs1`]mp_tac) >>
+  simp[] >>
+  disch_then(qx_choosel_then[`c1`]strip_assume_tac) >>
+  simp[Abbr`cs1`,Once SWAP_REVERSE] >>
+  simp[EVERY_MAP] >> fs[] >>
+  Q.PAT_ABBREV_TAC`cs1 = compiler_result_out_fupd X Y` >>
+  qmatch_assum_abbrev_tac`(compile_print_vals types map vs cs1').next_label = X` >>
+  `cs1' = cs1` by (
+    simp[Abbr`cs1`,Abbr`cs1'`,compiler_result_component_equality] ) >>
+  fs[Abbr`cs1'`] >> pop_assum kall_tac >>
+  conj_tac >- (
+    rpt(match_mp_tac code_labels_ok_cons>>simp[])>>
+    match_mp_tac code_labels_ok_append>>simp[IMPLODE_EXPLODE_I]>>
+    rpt(match_mp_tac code_labels_ok_append>>simp[]>>(TRY conj_tac)>>TRY(simp[code_labels_ok_def,uses_label_thm]>>NO_TAC))) >>
+  rpt gen_tac >>
+  strip_tac >>
+  fs[IMPLODE_EXPLODE_I] >>
+  `bs.code = bc0 ++ (MAP PrintC ("val "++v++":"++tystr types v++" = ")) ++ [Gread n;Print;PrintC(#"\n")] ++ c1` by (
+    simp[] ) >>
+  qmatch_assum_abbrev_tac`bs.code = bc0 ++ l1 ++ l2 ++ c1` >>
+  `bc_next^* bs (bs with <|pc:=next_addr bs.inst_length (bc0++l1)
+                          ;output:=STRCAT bs.output ("val "++v++":"++tystr types v++" = ")|>)` by (
+    match_mp_tac MAP_PrintC_thm >>
+    qexists_tac`"val "++v++":"++tystr types v++" = "`>>
+    qexists_tac`bc0` >>
+    simp[Abbr`l1`] ) >>
+  qmatch_assum_abbrev_tac`bc_next^* bs bs1` >>
+  `bc_fetch bs1 = SOME (Gread n)` by (
+    match_mp_tac bc_fetch_next_addr >>
+    simp[Abbr`bs1`] >>
+    qexists_tac`bc0++l1` >>
+    simp[Abbr`l2`] ) >>
+  `bc_next^* bs1 (bs1 with <|pc:=next_addr bs.inst_length(bc0++l1++l2)
+                            ;output := STRCAT bs1.output (print_bv bv)++"\n"|>)` by (
+    simp[RTC_eq_NRC] >>
+    qexists_tac`SUC(SUC(SUC 0))` >>
+    simp[NRC] >>
+    qho_match_abbrev_tac`∃z. bc_next bs1 z ∧ P z` >>
+    simp[bc_eval1_thm,bc_eval1_def,bump_pc_def] >>
+    simp[Abbr`bs1`,bc_eval_stack_def,EL_APPEND1]>>
+    fs[compilerLibTheory.el_check_def] >>
+    simp[Abbr`P`]>>
+    qho_match_abbrev_tac`∃z. bc_next bs1 z ∧ P z` >>
+    `bc_fetch bs1 = SOME Print` by (
+      match_mp_tac bc_fetch_next_addr >>
+      qexists_tac`bc0++l1++[HD l2]` >>
+      simp[Abbr`bs1`,Abbr`l2`] >>
+      simp[FILTER_APPEND,SUM_APPEND] ) >>
+    simp[bc_eval1_thm,bc_eval1_def,bump_pc_def]>>
+    simp[Abbr`bs1`]>>
+    simp[Abbr`P`] >>
+    qmatch_abbrev_tac`bc_next bs1 bs2` >>
+    `bc_fetch bs1 = SOME (PrintC(#"\n"))` by (
+      match_mp_tac bc_fetch_next_addr >>
+      qexists_tac`bc0++l1++FRONT l2` >>
+      simp[Abbr`bs1`,Abbr`l2`] >>
+      simp[FILTER_APPEND,SUM_APPEND] ) >>
+    simp[bc_eval1_thm,bc_eval1_def,bump_pc_def] >>
+    simp[Abbr`bs1`,Abbr`bs2`,bc_state_component_equality,IMPLODE_EXPLODE_I] >>
+    simp[FILTER_APPEND,SUM_APPEND,Abbr`l2`] ) >>
+  qmatch_assum_abbrev_tac`bc_next^* bs1 bs2` >>
+  `bc_next^* bs bs2` by metis_tac[RTC_TRANSITIVE,transitive_def] >>
+  pop_assum mp_tac >>
+  rpt(qpat_assum`bc_next^* a Y`kall_tac) >>
+  first_x_assum(qspecl_then[`bs2`,`bc0++l1++l2`,`ys`]mp_tac) >>
+  simp[Abbr`bs2`,Abbr`bs1`,ADD1] >>
+  strip_tac >>
+  qmatch_assum_abbrev_tac`bc_next^* bs1 bs2` >>
+  strip_tac >>
+  qmatch_abbrev_tac`bc_next^* bs bs2'` >>
+  `bs2' = bs2` by (
+    simp[Abbr`bs2`,Abbr`bs2'`,bc_state_component_equality,Abbr`l1`] >>
+    conj_tac >- (
+      simp[SUM_APPEND,FILTER_APPEND] ) >>
+    simp[print_bv_str_def]) >>
+  metis_tac[RTC_TRANSITIVE,transitive_def] )
+
+val _ = Parse.overload_on("print_ctor",``λx. STRCAT x " = <constructor>\n"``)
+val _ = Parse.overload_on("print_ctors",``λls. FLAT (MAP (λ(x,y). print_ctor x) ls)``)
+
+val compile_print_ctors_thm = store_thm("compile_print_ctors_thm",
+  ``∀ls cs. let cs' = compile_print_ctors ls cs in
+    ∃code. cs'.out = REVERSE code ++ cs.out
+      ∧ EVERY ($~ o is_Label) code
+      ∧ code_labels_ok code
+      ∧ cs'.next_label = cs.next_label ∧
+      ∀bs bc0.
+      bs.code = bc0 ++ code
+      ∧ bs.pc = next_addr bs.inst_length bc0
+      ⇒
+      let bs' = bs with <|pc := next_addr bs.inst_length bs.code
+           ; output := STRCAT bs.output (print_ctors ls)|> in
+      bc_next^* bs bs'``,
+  Induct >- (
+    simp[compile_print_ctors_def,Once SWAP_REVERSE] >>
+    rw[] >> simp[Once RTC_CASES1] >> simp[bc_state_component_equality] ) >>
+  qx_gen_tac`x` >> PairCases_on`x` >>
+  simp[compile_print_ctors_def,FOLDL_emit_thm,IMPLODE_EXPLODE_I] >>
+  rw[] >>
+  Q.PAT_ABBREV_TAC`cs1 = compiler_result_out_fupd x y` >>
+  first_x_assum(qspec_then`cs1`mp_tac) >>
+  simp[] >>
+  disch_then(Q.X_CHOOSE_THEN`c1`strip_assume_tac) >>
+  simp[Abbr`cs1`,Once SWAP_REVERSE,EVERY_MAP] >> fs[] >>
+  qmatch_assum_abbrev_tac`(compile_print_ctors ls cs1).next_label = X` >>
+  conj_tac >- (
+    match_mp_tac code_labels_ok_append >> simp[]>>
+    match_mp_tac code_labels_ok_append >> simp[]>>
+    rpt(match_mp_tac code_labels_ok_cons >> simp[]) ) >>
+  qmatch_abbrev_tac`((compile_print_ctors ls cs1').next_label = X) ∧ Y` >>
+  `cs1' = cs1` by (
+    simp[Abbr`cs1`,Abbr`cs1'`,compiler_result_component_equality] ) >>
+  simp[Abbr`X`,Abbr`Y`] >>
+  rpt strip_tac >>
+  qmatch_assum_abbrev_tac`bs.code = bc0 ++ l1 ++ l2 ++ c1` >>
+  `bc_next^* bs (bs with <|pc := next_addr bs.inst_length (bc0++l1++l2)
+                          ;output := bs.output ++ (x0++" = <constructor>\n")|>)` by (
+    match_mp_tac MAP_PrintC_thm >>
+    qexists_tac`x0 ++ " = <constructor>\n"` >>
+    qexists_tac`bc0` >>
+    simp[Abbr`l1`,Abbr`l2`] ) >>
+  qmatch_assum_abbrev_tac`bc_next^* bs bs1` >>
+  first_x_assum(qspecl_then[`bs1`,`bc0++l1++l2`]mp_tac) >>
+  simp[Abbr`bs1`] >>
+  strip_tac >>
+  qmatch_assum_abbrev_tac`bc_next^* bs bs1` >>
+  qmatch_assum_abbrev_tac`bc_next^* bs1' bs2` >>
+  `bs1' = bs1` by (
+    simp[Abbr`bs1'`,Abbr`bs1`,bc_state_component_equality] ) >>
+  qmatch_abbrev_tac`bc_next^* bs bs3` >>
+  `bs2 = bs3` by (
+    simp[Abbr`bs3`,bc_state_component_equality,semanticPrimitivesTheory.id_to_string_def] ) >>
+  metis_tac[RTC_TRANSITIVE,transitive_def])
+
+val compile_print_dec_thm = store_thm("compile_print_dec_thm",
+  ``∀types map d cs. let cs' = compile_print_dec types map d cs in
+      ∃code. cs'.out = REVERSE code ++ cs.out
+        ∧ EVERY ($~ o is_Label) code
+        ∧ cs'.next_label = cs.next_label
+        ∧ code_labels_ok code ∧
+      ∀bs bc0 bvs.
+      bs.code = bc0 ++ code
+      ∧ bs.pc = next_addr bs.inst_length bc0
+      ∧ LIST_REL
+        (λv bv. ∃n. FLOOKUP map v = SOME n ∧ el_check n bs.globals = SOME (SOME bv) ∧ can_Print bv)
+        (new_dec_vs d) bvs
+      ⇒
+      let str =
+        case d of
+        | Dtype ts => print_envC ([],build_tdefs NONE ts)
+        | Dexn cn ts => print_envC ([],[(cn, (LENGTH ts, TypeExn))])
+        | d => print_bv_list types (new_dec_vs d) bvs in
+      let bs' = bs with
+        <|pc := next_addr bs.inst_length (bc0++code)
+         ;output := bs.output ++ str|> in
+      bc_next^* bs bs'``,
+  Cases_on`d` >- (
+    simp[compile_print_dec_def] >>
+    rw[] >>
+    qspecl_then[`pat_bindings p []`,`types`, `map`,`cs`]mp_tac compile_print_vals_thm >>
+    simp[] >> rw[] >> simp[])
+  >- (
+    simp[compile_print_dec_def] >>
+    rw[] >>
+    Q.PAT_ABBREV_TAC`vs:string list = MAP X l` >>
+    qspecl_then[`vs`,`types`,`map`,`cs`]mp_tac compile_print_vals_thm >>
+    simp[] >> rw[] >> simp[] >> rpt gen_tac >> strip_tac >>
+    first_x_assum(qspecl_then[`bs`,`bc0`,`bvs`]mp_tac) >>
+    `vs = MAP FST l` by (
+      simp[Abbr`vs`,MAP_EQ_f,FORALL_PROD] ) >>
+    simp[TAKE_LENGTH_ID_rwt])
+  >- (
+    simp[] >>
+    simp[compile_print_dec_def] >>
+    Induct_on`REVERSE l` >- (
+      simp[compile_print_types_def,Once SWAP_REVERSE] >>
+      simp[Once SWAP_REVERSE] >>
+      simp[print_envC_def,semanticPrimitivesTheory.build_tdefs_def,LENGTH_NIL] >>
+      rw[] >> simp[Once RTC_CASES1] >> simp[bc_state_component_equality] ) >>
+    qx_gen_tac`x` >> PairCases_on`x` >>
+    gen_tac >> (disch_then (assume_tac o SYM)) >>
+    simp[compile_print_types_def] >>
+    gen_tac >>
+    specl_args_of_then``compile_print_ctors``compile_print_ctors_thm mp_tac >>
+    simp[] >>
+    disch_then(qx_choosel_then[`c1`]strip_assume_tac) >>
+    Q.ISPEC_THEN`l`mp_tac SNOC_CASES >>
+    strip_tac >> fs[] >> rw[] >> fs[] >>
+    Q.PAT_ABBREV_TAC`cs1 = compile_print_ctors X cs` >>
+    first_x_assum(qspec_then`cs1`mp_tac) >>
+    simp[Abbr`cs1`] >>
+    disch_then(qx_choosel_then[`c2`]strip_assume_tac) >>
+    simp[] >>
+    simp[Once SWAP_REVERSE] >>
+    conj_tac >- (
+      simp[code_labels_ok_append]>>simp[] ) >>
+    rpt strip_tac >>
+    last_x_assum(qspecl_then[`bs with code := bc0 ++ c1`,`bc0`]mp_tac) >>
+    simp[] >> strip_tac >>
+    qmatch_assum_abbrev_tac`bc_next^* bs0 bs1` >>
+    `bc_next^* bs (bs1 with code := bs.code)` by (
+      match_mp_tac RTC_bc_next_append_code >>
+      map_every qexists_tac[`bs0`,`bs1`] >>
+      simp[Abbr`bs0`,Abbr`bs1`,bc_state_component_equality] ) >>
+    first_x_assum(qspecl_then[`bs1 with code := bs.code`]mp_tac) >>
+    simp[Abbr`bs1`] >>
+    simp[LENGTH_NIL] >>
+    strip_tac >>
+    qmatch_assum_abbrev_tac`bc_next^* bs1' bs2` >>
+    qmatch_assum_abbrev_tac`bc_next^* bs bs1` >>
+    `bs1' = bs1` by (
+      simp[Abbr`bs1`,Abbr`bs1'`] ) >>
+    qmatch_abbrev_tac`bc_next^* bs bs2'` >>
+    `bs2' = bs2` by (
+      simp[Abbr`bs2`,Abbr`bs2'`] >>
+      simp[bc_state_component_equality] >>
+      simp[semanticPrimitivesTheory.build_tdefs_def,print_envC_def] >>
+      simp[MAP_REVERSE,MAP_MAP_o,combinTheory.o_DEF] >>
+      simp[UNCURRY,astTheory.mk_id_def] >>
+      simp[LAMBDA_PROD] ) >>
+    metis_tac[RTC_TRANSITIVE,transitive_def])
+  >- (
+    simp[] >>
+    simp[compile_print_dec_def] >>
+    simp[compile_print_types_def] >>
+    rw[] >>
+    qspecl_then[`[s,l]`,`cs`]mp_tac (INST_TYPE[alpha|->``:t list``]compile_print_ctors_thm) >>
+    simp[] >> rw[] >> simp[] >>
+    simp[print_envC_def]))
+
+val only_chars_lemma = prove(
+  ``∀s. only_chars (MAP (Number o $& o ORD) s)``,
+  Induct >> simp [only_chars_def,is_char_def,stringTheory.ORD_BOUND]);
+
+val Cv_bv_can_Print = save_thm("Cv_bv_can_Print",prove(
+  ``(∀Cv bv. Cv_bv pp Cv bv ⇒ can_Print bv) ∧
+    (∀bvs ce env defs. benv_bvs pp bvs ce env defs ⇒ T)``,
+  ho_match_mp_tac Cv_bv_ind >> simp[only_chars_lemma,only_chars_def] >>
+  simp[EVERY2_EVERY,EVERY_MEM,FORALL_PROD] >> rw[] >>
+  rfs[MEM_ZIP,GSYM LEFT_FORALL_IMP_THM,MEM_EL])
+  |> CONJUNCT1)
+
+val new_top_vs_def = Define`
+  (new_top_vs (Tdec dec) = new_dec_vs dec) ∧
+  (new_top_vs (Tmod _ _ _) = [])`
+
+val between_labels_def = Define`
+  between_labels bc l1 l2 ⇔
+  ALL_DISTINCT (FILTER is_Label bc) ∧
+  EVERY (between l1 l2) (MAP dest_Label (FILTER is_Label bc)) ∧
+  l1 ≤ l2`
+
+val good_labels_def = Define`
+  good_labels nl code ⇔
+    ALL_DISTINCT (FILTER is_Label code) ∧
+    EVERY (combin$C $< nl o dest_Label) (FILTER is_Label code)`
+
+val compile_print_top_thm = store_thm("compile_print_top_thm",
+  ``∀tys map t cs.
+    let cs' = compile_print_top tys map t cs in
+    ∃code.
+      cs'.out = REVERSE code ++ cs.out ∧
+      between_labels code cs.next_label cs'.next_label ∧
+      code_labels_ok code ∧
+      ∀bs bc0 st0 tag bv bvs.
+        bs.code = bc0 ++ code ∧
+        good_labels cs.next_label bc0 ∧
+        bs.pc = next_addr bs.inst_length bc0 ∧
+        bs.stack = (Block(block_tag+tag)(if tag = none_tag then [] else [bv]))::st0 ∧
+        (tag ≠ none_tag ⇒ can_Print bv) ∧
+        (∀d. tag = none_tag ∧ IS_SOME tys ∧ t = Tdec d ⇒
+         LIST_REL
+         (λv bv. ∃n. FLOOKUP map v = SOME n ∧ el_check n bs.globals = SOME (SOME bv) ∧ can_Print bv)
+         (new_dec_vs d) bvs)
+        ⇒ ∃pc.
+        (let str =
+          if tag ≠ none_tag then "raise " ++ print_bv bv ++ "\n" else
+          (case tys of NONE => ""
+          | SOME types => (case t of
+            | Tmod mn _ _ => "structure "++mn++" = <structure>\n"
+            | Tdec d => (case d of
+              | Dtype ts => print_envC ([],build_tdefs NONE ts)
+              | Dexn cn ts => print_envC ([],[(cn, (LENGTH ts, TypeExn))])
+              | d => print_bv_list types (new_dec_vs d) bvs))) in
+         let bs' = bs with <| pc := pc
+                            ; stack := st0
+                            ; output := bs.output ++ str |> in
+          bc_next^* bs bs' ∧
+          bc_fetch bs' = SOME (Stop (tag = none_tag)))``,
+  Cases_on`tys` >> Cases_on`t` >>
+  simp[compile_print_top_def,FOLDL_emit_thm] >>
+  rpt gen_tac >> simp[Once SWAP_REVERSE] >>
+  TRY (
+    specl_args_of_then``compile_print_dec``compile_print_dec_thm mp_tac >>
+    simp[] >> strip_tac >> simp[Once SWAP_REVERSE] ) >>
+  (conj_tac >- (
+     EVAL_TAC >>
+     REWRITE_TAC[FILTER_APPEND] >>
+     simp[MEM_FILTER,EVERY_FILTER,EVERY_MAP,MEM_MAP] >>
+     REWRITE_TAC[FILTER_APPEND] >> EVAL_TAC >>
+     simp[ALL_DISTINCT_APPEND,MEM_FILTER,MEM_MAP] >>
+     simp[FILTER_MAP,combinTheory.o_DEF] >>
+     fs[GSYM FILTER_EQ_NIL,combinTheory.o_DEF] >>
+     fs[FILTER_EQ_NIL,EVERY_MEM,is_Label_rwt,PULL_EXISTS] >>
+     CCONTR_TAC >> fs[] >> res_tac >> fs[])) >>
+  (conj_tac >-
+    (rpt(match_mp_tac code_labels_ok_cons >> simp[]) >>
+     EVAL_TAC >> simp[MEM_MAP] >>
+     rator_x_assum`code_labels_ok`mp_tac >>
+     EVAL_TAC >> metis_tac[])) >>
+  rpt gen_tac >> strip_tac >>
+  Q.PAT_ABBREV_TAC`str:string = if tag ≠ none_tag then X else Y` >>
+  (`bc_fetch bs = SOME(Stack(Load 0))` by (
+     match_mp_tac bc_fetch_next_addr >>
+     qexists_tac`bc0` >> simp[] )) >>
+  srw_tac[DNF_ss][Once RTC_CASES1] >> disj2_tac >>
+  simp[bc_eval1_thm,bc_eval1_def,bc_eval_stack_def,bump_pc_def] >>
+  qho_match_abbrev_tac`∃p. bc_next^* bs1 (bs2 p) ∧ P p` >>
+  `bc_fetch bs1 = SOME(Stack(TagEq(block_tag+none_tag)))` by (
+    match_mp_tac bc_fetch_next_addr >>
+    simp_tac (srw_ss()) [Abbr`bs1`] >>
+    qexists_tac`TAKE (LENGTH bc0 + 1) bs.code` >>
+    simp[TAKE_APPEND1,TAKE_APPEND2,SUM_APPEND,FILTER_APPEND,IMPLODE_EXPLODE_I] >>
+    NO_TAC) >>
+  srw_tac[DNF_ss][Once RTC_CASES1] >> disj2_tac >>
+  simp[bc_eval1_thm,bc_eval1_def,bump_pc_def] >>
+  simp[Abbr`bs1`,bc_eval_stack_def] >>
+  qho_match_abbrev_tac`∃p. bc_next^* bs1 (bs2 p) ∧ P p` >>
+  `bc_fetch bs1 = SOME(JumpIf (Lab cs.next_label))` by (
+    match_mp_tac bc_fetch_next_addr >>
+    simp_tac (srw_ss()) [Abbr`bs1`] >>
+    qexists_tac`TAKE (LENGTH bc0 + 2) bs.code` >>
+    simp[TAKE_APPEND1,TAKE_APPEND2,SUM_APPEND,FILTER_APPEND] >>
+    NO_TAC) >>
+  srw_tac[DNF_ss][Once RTC_CASES1] >> disj2_tac >>
+  simp[bc_eval1_thm,bc_eval1_def,bump_pc_def] >>
+  simp[Abbr`bs1`] >>
+  simp[PULL_EXISTS,bc_find_loc_def] >>
+  exists_suff_gen_then mp_tac bc_find_loc_aux_ALL_DISTINCT >>
+  disch_then(qspec_then`LENGTH bc0 + 13`mp_tac o CONV_RULE (RESORT_FORALL_CONV(sort_vars["k"]))) >>
+  disch_then exists_suff_tac >>
+  simp[EL_APPEND1,EL_APPEND2,RIGHT_EXISTS_AND_THM] >>
+  (conj_tac >- (
+     rator_x_assum`good_labels`mp_tac >>
+     TRY(rator_x_assum`code_labels_ok`mp_tac) >>
+     TRY(qpat_assum`EVERY ($~ o is_Label) X`mp_tac) >>
+     rpt(pop_assum kall_tac) >>
+     simp[GSYM FILTER_EQ_NIL,combinTheory.o_DEF,IMPLODE_EXPLODE_I] >>
+     REWRITE_TAC[FILTER_APPEND] >>
+     EVAL_TAC >> rpt strip_tac >>
+     fsrw_tac[ARITH_ss][ALL_DISTINCT_APPEND,MEM_FILTER,is_Label_rwt,PULL_EXISTS,EVERY_MEM,FILTER_MAP] >>
+     fs[FILTER_EQ_NIL,EVERY_MEM,is_Label_rwt,PULL_FORALL,combinTheory.o_DEF,MEM_MAP] >>
+     rw[] >> spose_not_then strip_assume_tac >> res_tac >> DECIDE_TAC )) >>
+  (reverse(Cases_on`tag=none_tag`>>fs[]) >- (
+     rfs[bc_fetch_def] >>
+     qho_match_abbrev_tac`∃p. bc_next^* bs1 (bs2 p) ∧ P p` >>
+     `bc_fetch bs1 = SOME(Stack(El 0))` by (
+       match_mp_tac bc_fetch_next_addr >>
+       simp_tac (srw_ss()) [Abbr`bs1`] >>
+       qexists_tac`TAKE (LENGTH bc0 + 3) bs.code` >>
+       simp[TAKE_APPEND1,TAKE_APPEND2,SUM_APPEND,FILTER_APPEND] >>
+       NO_TAC) >>
+     srw_tac[DNF_ss][Once RTC_CASES1] >> disj2_tac >>
+     simp[bc_eval1_thm,bc_eval1_def,bump_pc_def] >>
+     simp[Abbr`bs1`,bc_eval_stack_def] >>
+     qho_match_abbrev_tac`∃p. bc_next^* bs1 (bs2 p) ∧ P p` >>
+     qsuff_tac`∃bs3 p. bc_next^* bs1 bs3 ∧ bc_next^* bs3 (bs2 p) ∧ P p` >- metis_tac[RTC_TRANSITIVE,transitive_def] >>
+     exists_suff_gen_then (qspec_then`"raise "`mp_tac) MAP_PrintC_thm >>
+     simp[] >> disch_then(qspec_then`bs1`mp_tac) >>
+     simp[Abbr`bs1`] >>
+     disch_then(qspec_then`TAKE (LENGTH bc0 + 4) bs.code`mp_tac o CONV_RULE SWAP_FORALL_CONV) >>
+     simp[TAKE_APPEND1,TAKE_APPEND2] >>
+     discharge_hyps >- ( simp[SUM_APPEND,FILTER_APPEND] ) >>
+     qmatch_abbrev_tac`bc_next^* bs1' bs3 ⇒ Z` >>
+     strip_tac >> simp[Abbr`Z`] >> qexists_tac`bs3` >>
+     qho_match_abbrev_tac`∃p. bc_next^* bs1 bs3 ∧ bc_next^* bs3 (bs2 p) ∧ P p` >>
+     `bs1' = bs1` by (
+       simp[Abbr`bs1`,Abbr`bs1'`,bc_state_component_equality] >>
+       simp[SUM_APPEND,FILTER_APPEND] ) >>
+     rw[] >>
+     `bc_fetch bs3 = SOME(Print)` by (
+       match_mp_tac bc_fetch_next_addr >>
+       simp_tac (srw_ss()) [Abbr`bs3`] >>
+       qexists_tac`TAKE (LENGTH bc0 + 10) bs.code` >>
+       simp[TAKE_APPEND1,TAKE_APPEND2,SUM_APPEND,FILTER_APPEND] ) >>
+     srw_tac[DNF_ss][Once RTC_CASES1] >> disj2_tac >>
+     simp[bc_eval1_thm,bc_eval1_def,bump_pc_def] >>
+     simp[Abbr`bs3`,Abbr`bs1`] >>
+     qho_match_abbrev_tac`∃p. bc_next^* bs1 (bs2 p) ∧ P p` >>
+     qsuff_tac`∃bs3 p. bc_next^* bs1 bs3 ∧ bc_next^* bs3 (bs2 p) ∧ P p` >- metis_tac[RTC_TRANSITIVE,transitive_def] >>
+     exists_suff_gen_then (qspec_then`"\n"`mp_tac) MAP_PrintC_thm >>
+     simp[] >> disch_then(qspec_then`bs1`mp_tac) >>
+     simp[Abbr`bs1`] >>
+     disch_then(qspec_then`TAKE (LENGTH bc0 + 11) bs.code`mp_tac o CONV_RULE SWAP_FORALL_CONV) >>
+     simp[TAKE_APPEND1,TAKE_APPEND2] >>
+     discharge_hyps >- ( simp[SUM_APPEND,FILTER_APPEND] ) >>
+     qmatch_abbrev_tac`bc_next^* bs1' bs3 ⇒ Z` >>
+     strip_tac >> simp[Abbr`Z`] >> qexists_tac`bs3` >>
+     qho_match_abbrev_tac`∃p. bc_next^* bs1 bs3 ∧ bc_next^* bs3 (bs2 p) ∧ P p` >>
+     `bs1' = bs1` by (
+       simp[Abbr`bs1`,Abbr`bs1'`,bc_state_component_equality] >>
+       simp[SUM_APPEND,FILTER_APPEND] ) >>
+     rw[] >>
+     `bc_fetch bs3 = SOME(Stop F)` by (
+       match_mp_tac bc_fetch_next_addr >>
+       simp_tac (srw_ss()) [Abbr`bs3`] >>
+       qexists_tac`TAKE (LENGTH bc0 + 12) bs.code` >>
+       simp[TAKE_APPEND1,TAKE_APPEND2] >>
+       REWRITE_TAC[FILTER_APPEND] >>
+       EVAL_TAC >>
+       REWRITE_TAC[GSYM SUM_SUM_ACC] >>
+       simp[SUM_APPEND,FILTER_APPEND]) >>
+     srw_tac[DNF_ss][Once RTC_CASES1] >> disj1_tac >>
+     simp[Abbr`bs3`,Abbr`bs2`,bc_state_component_equality] >>
+     rfs[Abbr`P`,bc_fetch_def])) >>
+  TRY (
+    qho_match_abbrev_tac`∃p. bc_next^* bs1 (bs2 p) ∧ P p` >>
+    `bc_fetch bs1 = SOME(Stack Pop)` by (
+      match_mp_tac bc_fetch_next_addr >>
+      simp_tac (srw_ss()) [Abbr`bs1`] >>
+      qexists_tac`TAKE (LENGTH bc0 + 14) bs.code` >>
+      simp[TAKE_APPEND2] >>
+      simp_tac std_ss [FILTER_APPEND,SUM_APPEND] >>
+      EVAL_TAC ) >>
+    srw_tac[DNF_ss][Once RTC_CASES1] >> disj2_tac >>
+    simp[bc_eval1_thm,bc_eval1_def,bump_pc_def] >>
+    simp[Abbr`bs1`,bc_eval_stack_def] >>
+    srw_tac[DNF_ss][Once RTC_CASES1] >> disj1_tac >>
+    simp[Abbr`bs2`,bc_state_component_equality] >>
+    simp[Abbr`P`,TAKE_APPEND2] >>
+    match_mp_tac bc_fetch_next_addr >> simp[] >>
+    CONV_TAC SWAP_EXISTS_CONV >> qexists_tac`[]` >> simp[] >>
+    simp_tac std_ss [FILTER_APPEND,SUM_APPEND] >>
+    EVAL_TAC >> simp[ADD1] >>
+    REWRITE_TAC[GSYM SUM_SUM_ACC] >>
+    simp[SUM_APPEND] >> NO_TAC)
+  >- (
+    simp[TAKE_APPEND1,TAKE_APPEND2] >>
+    qho_match_abbrev_tac`∃p. bc_next^* bs1 (bs2 p) ∧ P p` >>
+    qsuff_tac`∃bs3 p. bc_next^* bs1 bs3 ∧ bc_next^* bs3 (bs2 p) ∧ P p` >- metis_tac[RTC_TRANSITIVE,transitive_def] >>
+    exists_suff_gen_then (qspec_then`"structure "++s++" = <structure>\n"`mp_tac) MAP_PrintC_thm >>
+    simp[] >> disch_then(qspec_then`bs1`mp_tac) >>
+    simp[Abbr`bs1`] >>
+    disch_then(qspec_then`TAKE (LENGTH bc0 + 14) bs.code`mp_tac o CONV_RULE SWAP_FORALL_CONV) >>
+    simp[TAKE_APPEND1,TAKE_APPEND2,IMPLODE_EXPLODE_I] >>
+    discharge_hyps >- ( REWRITE_TAC[FILTER_APPEND] >> EVAL_TAC) >>
+    qmatch_abbrev_tac`bc_next^* bs1' bs3 ⇒ Z` >>
+    strip_tac >> simp[Abbr`Z`] >> qexists_tac`bs3` >>
+    simp[RIGHT_EXISTS_AND_THM] >>
+    conj_tac >- (
+      qmatch_abbrev_tac`bc_next^* bs1 bs3` >>
+      `bs1' = bs1` by (
+        simp[Abbr`bs1`,Abbr`bs1'`,bc_state_component_equality] >>
+        REWRITE_TAC[FILTER_APPEND] >>
+        EVAL_TAC ) >>
+      rw[] ) >>
+    `bc_fetch bs3 = SOME(Stack Pop)` by (
+      match_mp_tac bc_fetch_next_addr >>
+      simp[Abbr`bs3`] >>
+      qexists_tac`TAKE (LENGTH bs.code - 2) bs.code` >>
+      simp[TAKE_APPEND1,TAKE_APPEND2,IMPLODE_EXPLODE_I] >>
+      REWRITE_TAC[FILTER_APPEND,FILTER_MAP,combinTheory.o_DEF] >>
+      EVAL_TAC >>
+      REWRITE_TAC[FILTER_APPEND,FILTER_MAP,combinTheory.o_DEF] >>
+      EVAL_TAC >>
+      simp[GSYM SUM_SUM_ACC,SUM_APPEND] ) >>
+    srw_tac[DNF_ss][Once RTC_CASES1] >> disj2_tac >>
+    simp[bc_eval1_thm,bc_eval1_def,bump_pc_def] >>
+    simp[Abbr`bs3`,bc_eval_stack_def] >>
+    srw_tac[DNF_ss][Once RTC_CASES1] >> disj1_tac >>
+    simp[Abbr`bs2`,bc_state_component_equality,Abbr`P`] >>
+    match_mp_tac bc_fetch_next_addr >> simp[] >>
+    CONV_TAC SWAP_EXISTS_CONV >> qexists_tac`[]` >> simp[] >>
+    simp[TAKE_APPEND1,TAKE_APPEND2,IMPLODE_EXPLODE_I] >>
+    REWRITE_TAC[FILTER_APPEND,FILTER_MAP,combinTheory.o_DEF] >>
+    EVAL_TAC >>
+    REWRITE_TAC[FILTER_APPEND,FILTER_MAP,combinTheory.o_DEF] >>
+    EVAL_TAC >>
+    simp[GSYM SUM_SUM_ACC,SUM_APPEND] ) >>
+  simp[TAKE_APPEND1,TAKE_APPEND2] >>
+  qho_match_abbrev_tac`∃p. bc_next^* bs1 (bs2 p) ∧ P p` >>
+  qmatch_assum_abbrev_tac`bs.code = bc0 ++ c1 ++ code ++ c2` >>
+  first_x_assum(qspecl_then[`bs1 with code := bc0 ++ c1 ++ code`,`bc0 ++ c1`,`bvs`]mp_tac) >>
+  simp[Abbr`bs1`] >>
+  discharge_hyps >- (
+    qunabbrev_tac`c1` >>
+    REWRITE_TAC[FILTER_APPEND] >>
+    EVAL_TAC ) >>
+  strip_tac >>
+  qmatch_assum_abbrev_tac`bc_next^* bs10 bs20` >>
+  qho_match_abbrev_tac`∃p. bc_next^* bs1 (bs2 p) ∧ P p` >>
+  `bs1 = bs10 with code := bs.code` by (
+    simp[Abbr`bs1`,Abbr`bs10`,bc_state_component_equality] >>
+    qunabbrev_tac`c1` >>
+    REWRITE_TAC[FILTER_APPEND] >>
+    EVAL_TAC ) >>
+  `bc_next^* bs1 (bs20 with code := bs.code)` by (
+    match_mp_tac RTC_bc_next_append_code >>
+    first_assum (match_exists_tac o concl) >>
+    simp[Abbr`bs10`,bc_state_component_equality] >>
+    simp[Abbr`bs20`] ) >>
+  qsuff_tac`∃bs3 p. bc_next^* bs1 bs3 ∧ bc_next^* bs3 (bs2 p) ∧ P p` >- metis_tac[RTC_TRANSITIVE,transitive_def] >>
+  HINT_EXISTS_TAC >> simp[] >> rw[] >>
+  qho_match_abbrev_tac`∃p. bc_next^* bs1 (bs2 p) ∧ P p` >>
+  `bc_fetch bs1 = SOME (Stack Pop)` by (
+    match_mp_tac bc_fetch_next_addr >>
+    simp[Abbr`bs1`,Abbr`bs20`] >>
+    qexists_tac`bc0 ++ c1 ++ code` >>
+    unabbrev_all_tac >> simp[] ) >>
+  srw_tac[DNF_ss][Once RTC_CASES1] >> disj2_tac >>
+  simp[bc_eval1_thm,bc_eval1_def,bump_pc_def] >>
+  simp[Abbr`bs1`,Abbr`bs20`,bc_eval_stack_def] >>
+  srw_tac[DNF_ss][Once RTC_CASES1] >> disj1_tac >>
+  simp[Abbr`bs2`,bc_state_component_equality,Abbr`P`] >>
+  unabbrev_all_tac >>
+  match_mp_tac bc_fetch_next_addr >> simp[] >>
+  CONV_TAC SWAP_EXISTS_CONV >> qexists_tac`[]` >> simp[] >>
+  REWRITE_TAC[FILTER_APPEND,FILTER_MAP,combinTheory.o_DEF] >>
+  EVAL_TAC >>
+  REWRITE_TAC[FILTER_APPEND,FILTER_MAP,combinTheory.o_DEF] >>
+  EVAL_TAC >>
+  simp[GSYM SUM_SUM_ACC,SUM_APPEND] )
+
+val _ = export_theory()
